high2/Zeta.High.Blum.fst
@@ -1,0 +1,222 @@
+module Zeta.High.Blum
+
+open Zeta.High.Thread
+
+let eac_state_transition_snoc
+  (#app #n:_)
+  (bk: base_key)
+  (il: eac_log app n {length il > 0})
+  : Lemma (ensures (let i = length il - 1 in
+                    let il' = prefix il i in
+                    let es' = eac_state_of_key bk il' in
+                    let es = eac_state_of_key bk il in
+                    let e = index il i in
+                    es' <> es ==> (
+                    match es', es with
+                    | EACInit, EACInStore m gk v ->
+                      AddM? e
+                    | EACInStore _ gk' _, EACEvictedBlum gk v t tid ->
+                      gk' = gk /\ is_blum_evict il i /\
+                      to_base_key gk = evict_slot (index il i) /\
+                      (let be = blum_evict_elem il i in
+                       let gke,ve = be.r in
+                       let open Zeta.MultiSetHashDomain in
+                       gke = gk /\ ve = v /\ be.t = t /\ be.tid = tid)
+                    | EACInStore _ _ _, EACEvictedMerkle _ _ ->
+                      EvictM? e
+                    | EACEvictedBlum gk v t tid, EACInStore _ gk' _ ->
+                      gk = gk' /\ is_blum_add il i /\
+                      to_base_key gk = add_slot (index il i) /\
+                      (let be = blum_add_elem il i in
+                       let open Zeta.MultiSetHashDomain in
+                       let gke, ve = be.r in
+                       gke = gk /\ ve = v /\ be.t = t /\ be.tid = tid
+                      )
+                    | EACEvictedMerkle _ _, EACInStore _ _ _ ->
+                      AddM? e
+                    | _ -> False)))
+  = admit()
+
+let eac_state_unchanged_snoc
+  (#app #n:_)
+  (ep: epoch)
+  (gk: key app)
+  (il: eac_log app n {length il > 0})
+  : Lemma (ensures (let i = length il - 1 in
+                    let il' = prefix il i in
+                    let bk = to_base_key gk in
+                    let es' = eac_state_of_key bk il' in
+                    let es = eac_state_of_key bk il in
+                    es' = es ==> (not (is_blum_add_of_key ep gk il i) /\
+                                  not (is_blum_evict_of_key ep gk il i))))
+  = admit()
+
+let rec evict_add_count_rel
+  (#app #n:_)
+  (ep: epoch)
+  (gk: key app)
+  (il: eac_log app n)
+  : Lemma (ensures(match eac_state_of_gkey gk il with
+                   | EACFail -> False
+                   | EACInit
+                   | EACInStore _ _ _
+                   | EACEvictedMerkle _ _ ->
+                     size (k_add_set ep gk il) = size (k_evict_set ep gk il)
+                   | EACEvictedBlum gke _ t _ ->
+                     if t.e = ep && gke = gk then
+                       size (k_add_set ep gk il) + 1 = size (k_evict_set ep gk il)
+                     else
+                       size (k_add_set ep gk il) = size (k_evict_set ep gk il)))
+          (decreases (length il))
+  = let bk = to_base_key gk in
+    if length il = 0
+    then (
+      k_add_set_empty ep gk il;
+      k_evict_set_empty ep gk il;
+      eac_state_empty bk il
+    )
+    else (
+      let i = length il - 1 in
+      let il' = prefix il  i in
+      k_add_set_snoc ep gk il;
+      k_evict_set_snoc ep gk il;
+      evict_add_count_rel ep gk il';
+      eac_state_transition_snoc bk il;
+      let es = eac_state_of_key bk il in
+      let es' = eac_state_of_key bk il' in
+      if es = es' then eac_state_unchanged_snoc ep gk il
+      else ()
+    )
+
+let evict_elem_fixes_eac_state_key
+  (#app #n:_)
+  (il: eac_log app n)
+  (i: seq_index il {is_blum_evict il i})
+  : Lemma (ensures (let be = blum_evict_elem il i in
+                    let gk,_ = be.r in
+                    let bk = to_base_key gk in
+                    let es = eac_state_of_key bk il in
+                    is_eac_state_active bk il /\
+                    to_gen_key bk il = gk))
+  = admit()
+
+let eac_instore_addb_diff_elem
+  (#app #n:_)
+  (itsl: its_log app n)
+  (i: seq_index itsl{let itsli = prefix itsl i in
+                     is_blum_add itsl i /\
+                     is_eac itsli /\
+                     (let e = index itsl i in
+                      let k = add_slot e in
+                      let es = eac_state_of_key k itsli in
+                      EACInStore? es)})
+  : (be':ms_hashfn_dom app{let ep = be'.t.e in
+                           let as = add_set ep itsl in
+                           let es = evict_set ep itsl in
+                           let be = blum_add_elem itsl i in
+                           mem be' as > mem be' es /\
+                           be.t.e = ep})
+  = let itsli = prefix itsl i in
+    let itsli' = prefix itsl (i+1) in
+    let e = index itsl i in
+    let k = add_slot e in
+    let be = blum_add_elem itsl i in
+    let ep = be.t.e in
+    let gk,_ = be.r in
+
+    //assert(to_base_key gk = k);
+    evict_add_count_rel ep gk itsli;
+    //assert(size (k_add_set ep gk itsli) = size (k_evict_set ep gk itsli));
+    k_add_set_snoc ep gk itsli';
+    k_evict_set_snoc ep gk itsli';
+
+    let be' = diff_elem (k_add_set ep gk itsli') (k_evict_set ep gk itsli') in
+    k_add_set_correct ep gk itsli' be';
+    add_set_rel_k_add_set ep gk itsli' be';
+    evict_set_rel_k_evict_set ep gk itsli' be';
+    //assert(mem be' (add_set ep itsli') > mem be' (evict_set ep itsli'));
+
+    lemma_evict_before_add2 ep itsl (i+1) be';
+    be'
+
+let eac_evictedm_addb_diff_elem
+  (#app #n:_)
+  (itsl: its_log app n)
+  (i:seq_index itsl{let itsli = prefix itsl i in
+                    is_blum_add itsl i /\
+                    is_eac itsli /\
+                    (let e = index itsl i in
+                     let k = add_slot e in
+                     let es = eac_state_of_key k itsli in
+                     EACEvictedMerkle? es)})
+  : (be':ms_hashfn_dom app{let ep = be'.t.e in
+                           let as = add_set ep itsl in
+                           let es = evict_set ep itsl in
+                           let be = blum_add_elem itsl i in
+                           mem be' as > mem be' es /\
+                           be.t.e = ep})
+  = let itsli = prefix itsl i in
+    let itsli' = prefix itsl (i+1) in
+    let e = index itsl i in
+    let k = add_slot e in
+    let be = blum_add_elem itsl i in
+    let ep = be.t.e in
+    let gk,_ = be.r in
+
+    //assert(to_base_key gk = k);
+    evict_add_count_rel ep gk itsli;
+    //assert(size (k_add_set ep gk itsli) = size (k_evict_set ep gk itsli));
+    k_add_set_snoc ep gk itsli';
+    k_evict_set_snoc ep gk itsli';
+
+    let be' = diff_elem (k_add_set ep gk itsli') (k_evict_set ep gk itsli') in
+    k_add_set_correct ep gk itsli' be';
+    add_set_rel_k_add_set ep gk itsli' be';
+    evict_set_rel_k_evict_set ep gk itsli' be';
+    //assert(mem be' (add_set ep itsli') > mem be' (evict_set ep itsli'));
+
+    lemma_evict_before_add2 ep itsl (i+1) be';
+    be'
+
+let eac_evictedb_addb_diff_elem
+  (#app #n:_)
+  (itsl: its_log app n)
+  (i: seq_index itsl{let itsli = prefix itsl i in
+                     let itsli' = prefix itsl (i + 1) in
+                     is_blum_add itsl i /\
+                     is_eac itsli /\
+                     not (is_eac itsli') /\
+                     (let e = index itsl i in
+                      let k = add_slot e in
+                      let es = eac_state_of_key k itsli in
+                      EACEvictedBlum? es)})
+  : (be':ms_hashfn_dom app{let ep = be'.t.e in
+                           let as = add_set ep itsl in
+                           let es = evict_set ep itsl in
+                           let be = blum_add_elem itsl i in
+                           mem be' as > mem be' es /\
+                           be.t.e = ep})
+  = let itsli = prefix itsl i in
+    let itsli' = prefix itsl (i+1) in
+    let e = index itsl i in
+    let k = add_slot e in
+    let be = blum_add_elem itsl i in
+    let ep = be.t.e in
+    let gk,_ = be.r in
+
+    //assert(to_base_key gk = k);
+    evict_add_count_rel ep gk itsli;
+    admit()
+
+(* when the eac store is evicted, there exists a previous evict *)
+let previous_evict_of_eac_evicted
+  (#app #n:_)
+  (itsl: eac_log app n)
+  (k: base_key {EACEvictedBlum? (eac_state_of_key k itsl)})
+  : i:seq_index itsl{is_blum_evict itsl i /\
+                     (let be = blum_evict_elem itsl i in
+                      let EACEvictedBlum gk v t j = eac_state_of_key k itsl in
+                      let gk',v' = be.r in
+                      let open Zeta.MultiSetHashDomain in
+                      gk = gk' /\ v = v' /\ be.t = t /\ be.tid = j)}
+  = admit()
